coq/Parsing.v
@@ -10,218 +10,325 @@ Export Coq.Strings.String.
 Export Coq.Lists.List.ListNotations.
 
 Declare Custom Entry koika.
-Declare Custom Entry koika_args.
+
+(* This is the entry point to transition from normal
+  Coq (constr) to koika *)
+Notation "'{{' e '}}'" := (e) (e custom koika at level 200, format "'{{' '[v' '/' e '/' ']' '}}'").
+
+(* Koika_var *)
 Declare Custom Entry koika_var.
-Declare Custom Entry koika_types.
-Declare Custom Entry koika_branches.
-Declare Custom Entry koika_consts.
+Notation "a" := (ident_to_string a) (in custom koika_var at level 0, a constr at level 0, only parsing).
+Notation "a" := (a) (in custom koika_var at level 0, a constr at level 0, format "'[' a ']'", only printing).
+
+(* koika_binder *)
+Declare Custom Entry koika_binder.
+Notation "'(' x ':' y ')'" := (x%string, y : type) (in custom koika_binder at level 0, x custom koika_var, y constr).
+Notation "a .. b" := (cons a ..  (cons b nil) ..)  (in custom koika_binder at level 1, a custom koika_binder at next level, b custom koika_binder at next level).
+
+Notation "'fun' nm args ':' ret '=>' body" :=
+  (Build_InternalFunction nm%string args ret body)
+    (in custom koika at level 200, nm custom koika_var, args custom koika_binder, ret constr at level 0, right associativity, format "'[v' 'fun'  nm  args  ':'  ret  '=>' '/' body ']'").
+Notation "'fun' nm '()' ':' ret '=>' body" :=
+  (Build_InternalFunction nm%string nil ret body)
+    (in custom koika at level 200, nm custom koika_var, ret constr at level 0, right associativity, format "'[v' 'fun'  nm  '()'   ':'  ret  '=>' '/' body ']'").
+
+Notation "'assert' a 'in' c"          := (UIf a c (USugar (UConstBits Ob))) (in custom koika at level 200, right associativity, format "'[v' 'assert'  a '/' 'in'  c ']'").
+Notation "'assert' a 'else' b 'in' c" := (UIf a c b                       ) (in custom koika at level 200, right associativity, format "'[v' 'assert'  a '/' 'else'  b '/' 'in'  c ']'").
+Notation "'when' a 'do' t "           := (UIf a t (USugar (UConstBits Ob))) (in custom koika at level 200, right associativity, format "'[v' 'when'  a '/' 'do'  t '/' ']'").
+
+Notation "'let' a ':=' b 'in' c" := (UBind a b c) (in custom koika at level 200, a custom koika_var, right associativity, format "'[v' 'let'  a  ':='  b  'in' '/' c ']'").
+
+Notation "a ';' b" := (USeq a                        b) (in custom koika at level 90, b at level 200, format "'[v' a ';' '/' b ']'" ).
+Notation "a ';'"   := (USeq a (USugar (UConstBits Ob))) (in custom koika at level 90). (* trailing comma *)
+
+Print Custom Grammar koika.
+
+
+Notation "'set' a ':=' b" := (UAssign a b) (in custom koika at level 89, a custom koika_var, format "set  a  :=  b").
+
+Notation "'if' a 'then' t 'else' f" := (UIf a t f) (in custom koika at level 89, right associativity, format "'[v' 'if'  a '/' 'then'  t '/' 'else'  f ']'").
+Notation "'guard' '(' a ')' " := (UIf (UUnop (UBits1 UNot) a) (UFail (bits_t 0)) (USugar (UConstBits Ob))) (in custom koika at level 89, right associativity, format "guard ( a )").
+
+(* Inspired by cpp precedence  *)
+(* https://en.cppreference.com/w/cpp/language/operator_precedence *)
+(* TODO id really prefer to use || and && for logical operations and & | for bitwise *)
+(* Bit operations *)
+Notation "a  '||'  b"  := (UBinop (UBits2     UOr)              a b) (in custom koika at level 85).
+Notation "a  '^'  b"   := (UBinop (UBits2    UXor)              a b) (in custom koika at level 84).
+Notation "a  '&&'  b"  := (UBinop (UBits2    UAnd)              a b) (in custom koika at level 83).
+
+(* Comparisons *)
+Notation "a  '!='  b"  := (UBinop (UEq true)                    a b) (in custom koika at level 80).
+Notation "a  '=='  b"  := (UBinop (UEq false)                   a b) (in custom koika at level 80).
+
+Notation "a  '<'  b"   := (UBinop (UBits2 (UCompare false cLt)) a b) (in custom koika at level 79).
+Notation "a  '<s'  b"  := (UBinop (UBits2 (UCompare true  cLt)) a b) (in custom koika at level 79).
+Notation "a  '<='  b"  := (UBinop (UBits2 (UCompare false cLe)) a b) (in custom koika at level 79).
+Notation "a  '<s='  b" := (UBinop (UBits2 (UCompare true  cLe)) a b) (in custom koika at level 79).
+Notation "a  '>'  b"   := (UBinop (UBits2 (UCompare false cGt)) a b) (in custom koika at level 79).
+Notation "a  '>s'  b"  := (UBinop (UBits2 (UCompare true  cGt)) a b) (in custom koika at level 79).
+Notation "a  '>='  b"  := (UBinop (UBits2 (UCompare false cGe)) a b) (in custom koika at level 79).
+Notation "a  '>s='  b" := (UBinop (UBits2 (UCompare true  cGe)) a b) (in custom koika at level 79).
+
+(* Bit concatenation / shifts *)
+Notation "a  '++'  b"  := (UBinop (UBits2 UConcat)              a b) (in custom koika at level 75).
+Notation "a  '>>'  b"  := (UBinop (UBits2 ULsr)                 a b) (in custom koika at level 74).
+Notation "a  '>>>'  b" := (UBinop (UBits2 UAsr)                 a b) (in custom koika at level 74).
+Notation "a  '<<'  b"  := (UBinop (UBits2 ULsl)                 a b) (in custom koika at level 74).
+
+(* Arithmetic *)
+Notation "a  '+'  b"   := (UBinop (UBits2   UPlus)              a b) (in custom koika at level 70).
+Notation "a  '-'  b"   := (UBinop (UBits2  UMinus)              a b) (in custom koika at level 70).
+Notation "a  '*'  b"   := (UBinop (UBits2    UMul)              a b) (in custom koika at level 69).
+
+(* Unary operators *)
+Notation "'!' a"       := (UUnop (UBits1 UNot) a)                    (in custom koika at level 65, format "'!' a").
+
+(* Accessors *)
+Notation "a '[' b ']'"        := (UBinop (UBits2 USel)              a b) (in custom koika at level 60, format "'[' a [ b ] ']'").
+Notation "a '[' b ':+' c ']'" := (UBinop (UBits2 (UIndexedSlice c)) a b) (in custom koika at level 60, c constr at level 0, format "'[' a [ b ':+' c ] ']'").
+
+(* get field of struct *)
+Notation "a '.[' f ']'" := (UUnop  (UStruct1 (UGetField f)) a) (in custom koika at level 60, f custom koika_var).
+
+Notation "'`' a '`'" := (a) (in custom koika, a constr).
+Notation "'(' a ')'" := (a) (in custom koika, a custom koika, format "'[v' '(' a ')' ']'").
+
+Notation "'#' s" := (USugar (UConstBits s)) (in custom koika at level 0, s constr at level 0, only parsing).
+
+(* ========================================================================= *)
+(*                   Notations beginning with an identifier                  *)
+(* ========================================================================= *)
+(*
+Note:
+  All these notations need to be on the same level (here 0)
+  else the parser would match on the highest level first and
+  never even consider notations on a lower level.
+
+  Likewise, all these notations need to start with a variable
+  on the same level and in the same grammar (here a constr on level 0).
+  Only so the parser can parse this variable first and then decide
+  (depending on the following tokens) which notation matches.
+
+Note:
+  Some of the literal notations also start with an identifier.
+  Thus, the same restrictions apply.
+*)
+Notation "a" := (UVar (ident_to_string a)) (in custom koika at level 0, a constr at level 0, only parsing).
+Notation "a" := (UVar a) (in custom koika at level 0, a constr at level 0, only printing).
+
+(* Alternative shorter set syntax
+Note: expr is level 89 to stay below ';'
+*)
+Export (hints) IdentParsing.TC.
+Notation "a ':=' b" := (let aa := (TC.ident_to_string a) in UAssign aa b) (in custom koika at level 0, a constr at level 0, b custom koika at level 89, only parsing).
+Notation "a ':=' b" := (UAssign a b)                                      (in custom koika at level 0, a constr at level 0, b custom koika at level 89, only printing).
+
+
+(* Koika_args *)
+Declare Custom Entry koika_args.
+Notation "'(' x ',' .. ',' y ')'" := (cons x .. (cons y nil) ..)(in custom koika_args, x custom koika, y custom koika).
+Notation "'(' ')'" := nil (in custom koika_args).
+Notation "'()'"    := nil (in custom koika_args).
+
+Notation "fn args"                    := (USugar (UCallModule id       _ fn args))
+    (in custom koika at level 0, fn constr at level 0 , args custom koika_args, only parsing).
+
+Notation "instance  '.(' fn ')' args" := (USugar (UCallModule instance _ fn args))
+    (in custom koika at level 0, instance constr at level 0, fn constr, args custom koika_args).
+
+Notation "'{' fn '}' args"            := (USugar (UCallModule id       _ fn args))
+    (in custom koika at level 0, fn constr , args custom koika_args, only parsing).
+
+
+(* ========================================================================= *)
+(*                                  Literals                                 *)
+(* ========================================================================= *)
 
 (* Koika_consts *)
-Notation "'1'" :=
-  (Ob~1)
-    (in custom koika_consts at level 0).
-Notation "'0'" :=
-  (Ob~0)
-    (in custom koika_consts at level 0).
+Declare Custom Entry koika_consts.
+Notation "'1'" := (Ob~1) (in custom koika_consts at level 0).
+Notation "'0'" := (Ob~0) (in custom koika_consts at level 0).
+Notation "bs '~' '0'" := (Bits.cons false bs) (in custom koika_consts at level 1, left associativity, format "bs '~' '0'").
+Notation "bs '~' '1'" := (Bits.cons true bs)  (in custom koika_consts at level 1, left associativity, format "bs '~' '1'").
 
-Notation "bs '~' '0'" := (Bits.cons false bs) (in custom koika_consts at level 7, left associativity, format "bs '~' '0'").
-Notation "bs '~' '1'" := (Bits.cons true bs) (in custom koika_consts at level 7, left associativity, format "bs '~' '1'").
+Notation "'Ob' '~' number" := (USugar (UConstBits number))
+  (in custom koika at level 0, number custom koika_consts, format "'Ob' '~' number").
 
-Notation "'Ob' '~' number" :=
-  (USugar (UConstBits number))
-    (in custom koika at level 7, number custom koika_consts at level 99, format "'Ob' '~' number").
+(* koika bit vector literals *)
+From Coq Require BinaryString OctalString HexString HexadecimalString DecimalString.
 
+(* Unset Printing Notations.
+From Coq Require Ascii.
+
+Compute (list_ascii_of_string "_").
+Compute (String "_" EmptyString). *)
+
+Require Import Ascii.
+Local Fixpoint filters' (s : string) (a : ascii) : string :=
+  match s with
+  | EmptyString => EmptyString
+  | String c s' => if ascii_dec c a
+    then filters' s' a
+    else String c (filters' s' a)
+  end.
+Local Fixpoint filters (s : string) (l : list ascii) : string :=
+  match l with
+  | a :: l' => filters (filters' s a) l'
+  | [] => s
+  end.
+
+(* Coq's implementation just silently returns 0 on an invalid string -
+  for better error recognition these methods are redefined here returning option *)
+Local Fixpoint num_string_to_option_N' (s : string) (base : N) (convert : Ascii.ascii -> option N) (remainder : option N) : option N :=
+  match s with
+  | EmptyString => remainder
+  | String c s' => num_string_to_option_N' s' base convert
+    (match remainder, convert c with
+    | Some rem, Some c_v => Some (N.add (N.mul base rem) c_v)
+    | _, _ => None
+    end)
+  end.
+Local Definition num_string_to_option_N (s : string) (base : N) (convert : Ascii.ascii -> option N) : option N :=
+  match s with
+  | EmptyString => None
+  | String _ _ => num_string_to_option_N' s base convert (Some 0%N)
+  end.
+
+Local Definition bin_string_to_N s := (must (num_string_to_option_N s 2 BinaryString.ascii_to_digit)).
+Local Definition oct_string_to_N s := (must (num_string_to_option_N s 8 OctalString.ascii_to_digit)).
+Local Definition dec_string_to_N s := (must (option_map N.of_uint (DecimalString.NilZero.uint_of_string s))).
+Local Definition hex_string_to_N s := (must (num_string_to_option_N s 16 HexString.ascii_to_digit)).
+
+Local Definition len := String.length.
+Local Definition filt s := filters s ["_"; "'"]%char.
+
+Notation "num ':b' sz" := (let s := filt num in (USugar (UConstBits (Bits.of_N (sz <: nat)            (bin_string_to_N s))))) (in custom koika at level 0, num constr at level 0, sz constr at level 0, only parsing).
+Notation "num ':b'"    := (let s := filt num in (USugar (UConstBits (Bits.of_N ((len s) * 1)          (bin_string_to_N s))))) (in custom koika at level 0, num constr at level 0,                       only parsing).
+Notation "'0b' num sz" := (let s := filt num in (USugar (UConstBits (Bits.of_N (sz <: nat)            (bin_string_to_N s))))) (in custom koika at level 0, num constr at level 0, sz constr at level 0, format "'0b' num sz").
+Notation "'0b' num"    := (let s := filt num in (USugar (UConstBits (Bits.of_N ((len s) * 1)          (bin_string_to_N s))))) (in custom koika at level 0, num constr at level 0,                       only parsing).
+Notation "'0b' num"    := (let s := filt num in (USugar (UConstBits (Bits.of_N _                      (bin_string_to_N s))))) (in custom koika at level 0, num constr at level 0, only printing,        format "'0b' num").
+
+Notation "num ':o' sz" := (let s := filt num in (USugar (UConstBits (Bits.of_N (sz <: nat)            (oct_string_to_N s))))) (in custom koika at level 0, num constr at level 0, sz constr at level 0, only parsing).
+Notation "num ':o'"    := (let s := filt num in (USugar (UConstBits (Bits.of_N ((len s) * 3)          (oct_string_to_N s))))) (in custom koika at level 0, num constr at level 0,                       only parsing).
+Notation "'0o' num sz" := (let s := filt num in (USugar (UConstBits (Bits.of_N (sz <: nat)            (oct_string_to_N s))))) (in custom koika at level 0, num constr at level 0, sz constr at level 0, format "'0o' num sz").
+Notation "'0o' num"    := (let s := filt num in (USugar (UConstBits (Bits.of_N ((len s) * 3)          (oct_string_to_N s))))) (in custom koika at level 0, num constr at level 0,                       only parsing).
+Notation "'0o' num"    := (let s := filt num in (USugar (UConstBits (Bits.of_N _                      (oct_string_to_N s))))) (in custom koika at level 0, num constr at level 0, only printing,        format "'0o' num").
+
+Notation "num ':d' sz" := (let s := filt num in (USugar (UConstBits (Bits.of_N (sz <: nat)            (dec_string_to_N s))))) (in custom koika at level 0, num constr at level 0, sz constr at level 0, only parsing).
+Notation "num ':d'"    := (let s := filt num in (USugar (UConstBits (Bits.of_N (1 + (N.to_nat (N.log2 (dec_string_to_N s))))
+                                                            (dec_string_to_N s))))) (in custom koika at level 0, num constr at level 0,                       only parsing).
+Notation "'0d' num sz" := (let s := filt num in (USugar (UConstBits (Bits.of_N (sz <: nat)            (dec_string_to_N s))))) (in custom koika at level 0, num constr at level 0, sz constr at level 0, format "'0d' num sz").
+Notation "'0d' num"    := (let s := filt num in (USugar (UConstBits (Bits.of_N (1 + (N.to_nat (N.log2 (dec_string_to_N s))))
+                                                            (dec_string_to_N s))))) (in custom koika at level 0, num constr at level 0,                       only parsing).
+Notation "'0d' num"    := (let s := filt num in (USugar (UConstBits (Bits.of_N _                      (dec_string_to_N s))))) (in custom koika at level 0, num constr at level 0, only printing,        format "'0d' num").
+
+Notation "num ':h' sz" := (let s := filt num in (USugar (UConstBits (Bits.of_N (sz <: nat)            (hex_string_to_N s))))) (in custom koika at level 0, num constr at level 0, sz constr at level 0, only parsing).
+Notation "num ':h'"    := (let s := filt num in (USugar (UConstBits (Bits.of_N ((len s) * 4)          (hex_string_to_N s))))) (in custom koika at level 0, num constr at level 0,                       only parsing).
+Notation "'0x' num sz" := (let s := filt num in (USugar (UConstBits (Bits.of_N (sz <: nat)            (hex_string_to_N s))))) (in custom koika at level 0, num constr at level 0, sz constr at level 0, format "'0x' num sz").
+Notation "'0x' num"    := (let s := filt num in (USugar (UConstBits (Bits.of_N ((len s) * 4)          (hex_string_to_N s))))) (in custom koika at level 0, num constr at level 0,                       only parsing).
+Notation "'0x' num"    := (let s := filt num in (USugar (UConstBits (Bits.of_N _                      (hex_string_to_N s))))) (in custom koika at level 0, num constr at level 0, only printing,        format "'0x' num").
+
+(* legacy number format *)
 Notation "'|' a '`d' b '|'" :=
   (USugar (UConstBits (Bits.of_N (a<:nat) b%N)))
     (in custom koika, a constr at level 0 , b constr at level 0).
 
-(* Koika_args *)
-Declare Custom Entry koika_middle_args.
-Notation "x" := [x] (in custom koika_middle_args at level 0, x custom koika at level 99).
-Notation "x ',' y" := (app x y) (in custom koika_middle_args at level 1, x custom koika_middle_args, y custom koika_middle_args, right associativity).
+(* ========================================================================= *)
+(*                                Constructors                               *)
+(* ========================================================================= *)
 
-Notation "'()'"  := nil (in custom koika_args).
-(* Notation "'( )'"  := nil (in custom koika_args). *)
-Notation "'(' x ')'"  := x (in custom koika_args, x custom koika_middle_args).
-(* Koika_var *)
-Notation "a" := (ident_to_string a) (in custom koika_var at level 0, a constr at level 0, only parsing).
-Notation "a" := (a) (in custom koika_var at level 0, a constr at level 0, format "'[' a ']'", only printing).
+Declare Custom Entry koika_struct.
+Declare Custom Entry koika_struct_field.
+(* expr at level at level 89 to stay below koika's sequence (a ; b) *)
+Notation "f ':=' expr" := (f, expr) (in custom koika_struct_field at level 0, f custom koika_var, expr custom koika at level 89).
+Notation "a ';' b" := (cons a   b) (in custom koika_struct at level 0, a custom koika_struct_field, right associativity).
+Notation "a ';'"   := (cons a nil) (in custom koika_struct at level 0, a custom koika_struct_field). (* trailing comma *)
+Notation "a"       := (cons a nil) (in custom koika_struct at level 0, a custom koika_struct_field).
 
-(* Koika_types *)
-Notation " '(' x ':' y ')'" := (cons (prod_of_argsig {| arg_name := x%string; arg_type := y |}) nil) (in custom koika_types at level 60, x custom koika_var at level 0, y constr at level 12 ).
-Notation "a  b" := (app a b)  (in custom koika_types at level 95, a custom koika_types , b custom koika_types, right associativity).
+Notation "'struct' sig '{' '}'"        := (USugar (UStructInit sig []))
+  (in custom koika, sig constr at level 0).
+Notation "'struct' sig '{' fields '}'" := (USugar (UStructInit sig fields))
+  (in custom koika, sig constr at level 0, fields custom koika_struct).
+Notation "'enum' sig '{' mem '}'"      := (USugar (UConstEnum sig mem))
+  (in custom koika, sig constr at level 0, mem custom koika_var).
 
-(* Koika_branches *)
-Notation "x '=>' a " := (cons (x,a) nil) (in custom koika_branches at level 60, x custom koika at level 99, a custom koika at level 99).
-Notation "arg1 '|' arg2" := (app arg1 arg2) (in custom koika_branches at level 13, arg1 custom koika_branches, arg2 custom koika_branches, format "'[v' arg1 ']' '/' '|'  '[v' arg2 ']'").
 
-(* Koika *)
-Notation "'{{' e '}}'" := (e) (e custom koika at level 200, format "'{{' '[v' '/' e '/' ']' '}}'").
+Notation "sig '::{' '}'"        := (USugar (UStructInit sig []))
+  (in custom koika at level 0, sig constr at level 0).
+Notation "sig '::{' fields '}'" := (USugar (UStructInit sig fields))
+  (in custom koika at level 0, sig constr at level 0, fields custom koika_struct).
+Notation "sig '::<' mem '>'"    := (USugar (UConstEnum sig mem))
+  (in custom koika at level 0, sig constr at level 0, mem custom koika_var).
 
-Notation "'fail'" :=
-  (UFail (bits_t 0)) (in custom koika at level 1, format "'fail'").
-Notation "'fail' '(' t ')'" :=
-  (UFail (bits_t t)) (in custom koika at level 1, t constr at level 0, format "'fail' '(' t ')'").
-Notation "'fail' '@(' t ')'" :=
-  (UFail t)          (in custom koika at level 1, t constr at level 0 ,format "'fail' '@(' t ')'").
+
+(* ========================================================================= *)
+(*                        Closed Notations on level 0                        *)
+(* ========================================================================= *)
+
 Notation "'pass'" := (USugar (UConstBits Ob)) (in custom koika).
 Notation "'magic'" := (USugar UErrorInAst) (in custom koika).
 
-Notation "'let' a ':=' b 'in' c" := (UBind a b c) (in custom koika at level 91, a custom koika_var at level 1, right associativity, format "'[v' 'let'  a  ':='  b  'in' '/' c ']'").
-Notation "a ';' b" := (USeq a b) (in custom koika at level 90, format "'[v' a ';' '/' b ']'" ).
-Notation "'set' a ':=' b" := (UAssign a b) (in custom koika at level 89, a custom koika_var at level 1, format "'set'  a  ':='  b").
-Notation "'(' a ')'" := (a) (in custom koika at level 1, a custom koika, format "'[v' '(' a ')' ']'").
+Notation "'fail'"            := (UFail (bits_t 0)) (in custom koika, format "fail").
+Notation "'fail' '(' t ')'"  := (UFail (bits_t t)) (in custom koika, t constr, format "fail ( t )").
+Notation "'fail' '@(' t ')'" := (UFail t         ) (in custom koika, t constr, format "fail @( t )").
 
-Notation "instance  '.(' method ')' args" :=
-  (USugar (UCallModule instance _ method args))
-    (in custom koika at level 0, instance constr at level 0, method constr, args custom koika_args at level 99).
-Notation "'{' method '}' args" :=
-  (USugar (UCallModule id _ method args))
-    (in custom koika at level 1, method constr at level 200 , args custom koika_args at level 99, only parsing).
-Notation "method args" :=
-  (USugar (UCallModule id _ method args))
-    (in custom koika at level 0, method constr at level 0 , args custom koika_args at level 99, only parsing).
 
-Notation "a" := (UVar (ident_to_string a)) (in custom koika at level 0, a constr at level 0, only parsing).
-Notation "a" := (UVar a) (in custom koika at level 0, a constr at level 0, only printing).
+Notation "'read0' '(' reg ')' "           := (URead P0 reg)        (in custom koika, reg constr, format "read0 ( reg )").
+Notation "'read1' '(' reg ')' "           := (URead P1 reg)        (in custom koika, reg constr, format "read1 ( reg )").
+Notation "'write0' '(' reg ',' value ')'" := (UWrite P0 reg value) (in custom koika, reg constr, format "write0 ( reg ,  value )").
+Notation "'write1' '(' reg ',' value ')'" := (UWrite P1 reg value) (in custom koika, reg constr, format "write1 ( reg ,  value )").
 
-Notation "'read0' '(' reg ')' " := (URead P0 reg) (in custom koika at level 1, reg constr, format "'read0' '(' reg ')'").
-Notation "'read1' '(' reg ')' " := (URead P1 reg) (in custom koika at level 1, reg constr, format "'read1' '(' reg ')'").
-Notation "'write0' '(' reg ',' value ')'" :=
-  (UWrite P0 reg value)
-    (in custom koika at level 1, reg constr at level 13, format "'write0' '(' reg ',' value ')'").
-Notation "'write1' '(' reg ',' value ')'" :=
-  (UWrite P1 reg value)
-    (in custom koika at level 1, reg constr at level 13, format "'write1' '(' reg ',' value ')'").
 
-Notation "'if' a 'then' t 'else' f" := (UIf a t f) (in custom koika at level 86, right associativity, format "'[v' 'if'  a '/' 'then'  t '/' 'else'  f ']'").
-Notation "'guard' '(' a ')' " := (UIf (UUnop (UBits1 UNot) a) (UFail (bits_t 0)) (USugar (UConstBits Ob))) (in custom koika at level 86, right associativity, format "'guard' '(' a ')'").
-Notation "'when' a 'do' t " := (UIf a t (USugar (UConstBits Ob))) (in custom koika at level 91, right associativity, format "'[v' 'when'  a '/' 'do'  t '/' ']'").
-Notation "'assert' a 'in' c"          := (UIf a c (USugar (UConstBits Ob))) (in custom koika at level 91, a custom koika at level 200, right associativity, format "'[v' 'assert'  a '/' 'in'  c ']'").
-Notation "'assert' a 'else' b 'in' c" := (UIf a c b                       ) (in custom koika at level 91, a custom koika at level 200, right associativity, format "'[v' 'assert'  a '/' 'else'  b '/' 'in'  c ']'").
+Notation "'zeroExtend(' a ',' b ')'" :=  (UUnop (UBits1 (UZExtL b)) a) (in custom koika, b constr, format "'zeroExtend(' a ',' b ')'").
+Notation "'sext(' a ',' b ')'"       :=  (UUnop (UBits1 (USExt  b)) a) (in custom koika, b constr, format "'sext(' a ',' b ')'").
 
-Notation "a '&&' b" :=  (UBinop (UBits2 UAnd) a b) (in custom koika at level 80,  right associativity, format "a  '&&'  b").
-Notation "'!' a" := (UUnop (UBits1 UNot) a) (in custom koika at level 75, format "'!' a").
-Notation "a '||' b" :=  (UBinop (UBits2 UOr) a b) (in custom koika at level 85, format "a  '||'  b").
-Notation "'zeroExtend(' a ',' b ')'" :=  (UUnop (UBits1 (UZExtL b)) a) (in custom koika, b constr at level 0, format "'zeroExtend(' a ',' b ')'").
-Notation "'sext(' a ',' b ')'" :=  (UUnop (UBits1 (USExt b)) a) (in custom koika, b constr at level 0, format "'sext(' a ',' b ')'").
-Notation "'ignore(' a ')'" :=  (UUnop (UConv UIgnore) a) (in custom koika, a custom koika).
-Notation "'pack(' a ')'" :=  (UUnop (UConv UPack) a) (in custom koika, a custom koika).
-Notation "'unpack(' t ',' v ')'" :=  (UUnop (UConv (UUnpack t)) v) (in custom koika, t constr at level 11, v custom koika).
-Notation "a  '^'  b" :=  (UBinop (UBits2 UXor) a b) (in custom koika at level 85).
-Notation "a  '+'  b" :=  (UBinop (UBits2 UPlus) a b) (in custom koika at level 85).
-Notation "a  '-'  b" :=  (UBinop (UBits2 UMinus) a b) (in custom koika at level 85).
-Notation "a  '*'  b" := (UBinop (UBits2 UMul) a b) (in custom koika at level 84).
-Notation "a  '!='  b" := (UBinop (UEq true) a b) (in custom koika at level 79).
-Notation "a  '=='  b" :=  (UBinop (UEq false) a b) (in custom koika at level 79).
-Notation "a  '>>'  b" :=  (UBinop (UBits2 ULsr) a b) (in custom koika at level 79).
-Notation "a  '>>>'  b" :=  (UBinop (UBits2 UAsr) a b) (in custom koika at level 79).
-Notation "a  '<<'  b" :=  (UBinop (UBits2 ULsl) a b) (in custom koika at level 79).
-Notation "a  '<'  b" := (UBinop (UBits2 (UCompare false cLt)) a b) (in custom koika at level 79).
-Notation "a  '<s'  b" := (UBinop (UBits2 (UCompare true cLt)) a b) (in custom koika at level 79).
-Notation "a  '<='  b" := (UBinop (UBits2 (UCompare false cLe)) a b) (in custom koika at level 79).
-Notation "a  '<s='  b" := (UBinop (UBits2 (UCompare true cLe)) a b) (in custom koika at level 79).
-Notation "a  '>'  b" := (UBinop (UBits2 (UCompare false cGt)) a b) (in custom koika at level 79).
-Notation "a  '>s'  b" := (UBinop (UBits2 (UCompare true cGt)) a b) (in custom koika at level 79).
-Notation "a  '>='  b" := (UBinop (UBits2 (UCompare false cGe)) a b) (in custom koika at level 79).
-Notation "a  '>s='  b" := (UBinop (UBits2 (UCompare true cGe)) a b) (in custom koika at level 79).
-Notation "a '++' b" :=  (UBinop (UBits2 UConcat) a b) (in custom koika at level 80,  right associativity, format "a  '++'  b").
-Notation "a '[' b ']'" := (UBinop (UBits2 USel) a b) (in custom koika at level 75, format "'[' a [ b ] ']'").
-(* Notation "a '[' b ':' c ']'" := (UBinop (UBits2 (UIndexedSlice c)) a b) (in custom koika at level 75, c constr at level 0, format "'[' a [ b ':+' c ] ']'"). *)
-Notation "a '[' b ':+' c ']'" := (UBinop (UBits2 (UIndexedSlice c)) a b) (in custom koika at level 75, c constr at level 0, format "'[' a [ b ':+' c ] ']'").
-Notation "'`' a '`'" := ( a) (in custom koika at level 99, a constr at level 99).
-
-Notation "'fun' nm args ':' ret '=>' body" :=
-  {| int_name := nm%string;
-     int_argspec := args;
-     int_retSig := ret;
-     int_body := body |}
-    (in custom koika at level 99, nm custom koika_var at level 0, args custom koika_types, ret constr at level 0, body custom koika at level 99, format "'[v' 'fun'  nm  args  ':'  ret  '=>' '/' body ']'").
-Notation "'fun' nm '()' ':' ret '=>' body" :=
-  {| int_name := nm%string;
-     int_argspec := nil;
-     int_retSig := ret;
-     int_body := body |}
-    (in custom koika at level 99, nm custom koika_var at level 0, ret constr at level 0, body custom koika at level 99, format "'[v' 'fun'  nm  '()'   ':'  ret  '=>' '/' body ']'").
+Notation "'ignore(' a ')'"       :=  (UUnop (UConv     UIgnore) a) (in custom koika).
+Notation "'pack(' a ')'"         :=  (UUnop (UConv       UPack) a) (in custom koika).
+Notation "'unpack(' t ',' v ')'" :=  (UUnop (UConv (UUnpack t)) v) (in custom koika, t constr).
 
 (* Deprecated *)
-Notation "'call' instance method args" :=
+(* Notation "'call' instance method args" :=
   (USugar (UCallModule instance _ method args))
     (in custom koika at level 99, instance constr at level 0, method constr at level 0, args custom koika_args).
 Notation "'funcall' method args" :=
   (USugar (UCallModule id _ method args))
-    (in custom koika at level 98, method constr at level 0, args custom koika_args).
+    (in custom koika at level 98, method constr at level 0, args custom koika_args). *)
 Notation "'extcall' method '(' arg ')'" :=
   (UExternalCall method arg)
-    (in custom koika at level 98, method constr at level 0, arg custom koika).
-Notation "'call0' instance method " :=
+    (in custom koika, method constr at level 0).
+(* Notation "'call0' instance method " :=
   (USugar (UCallModule instance _ method nil))
     (in custom koika at level 98, instance constr at level 0, method constr).
 Notation "'funcall0' method " :=
   (USugar (UCallModule id _ method nil))
-    (in custom koika at level 98,  method constr at level 0).
+    (in custom koika at level 98,  method constr at level 0). *)
 
-Notation "'get' '(' v ',' f ')'" :=
-  (UUnop (UStruct1 (UGetField f)) v)
-    (in custom koika, v custom koika at level 13, f custom koika_var at level 0, format "'get' '(' v ','  f ')'").
-Notation "'getbits' '(' t ',' v ',' f ')'" :=
-  (UUnop (UStruct1 (UGetFieldBits t f)) v)
-    (in custom koika, t constr at level 11, v custom koika at level 13,
-        f custom koika_var at level 0,
-        format "'getbits' '(' t ','  v ','  f ')'").
-Notation "'subst' '(' v ',' f ',' a ')'" :=
-  (UBinop (UStruct2 (USubstField f)) v a)
-    (in custom koika, v custom koika at level 13, a custom koika at level 13, f custom koika_var at level 0, format "'subst' '(' v ','  f ',' a ')'").
-Notation "'substbits' '(' t ',' v ',' f ',' a ')'" :=
-  (UBinop (UStruct2 (USubstFieldBits t f)) v a)
-    (in custom koika, t constr at level 11, v custom koika at level 13,
-        a custom koika at level 13, f custom koika_var at level 0,
-        format "'substbits' '(' t ','  v ','  f ',' a ')'").
 
-Notation "'aref' '(' v ',' f ')'" :=
-  (UUnop (UArray1 (UGetElement f)) v)
-    (in custom koika, v custom koika at level 13, f constr at level 0, format "'aref' '(' v ','  f ')'").
-Notation "'arefbits' '(' t ',' v ',' f ')'" :=
-  (UUnop (UArray1 (UGetElementBits t f)) v)
-    (in custom koika, t constr at level 11, v custom koika at level 13,
-        f constr at level 0,
-        format "'arefbits' '(' t ','  v ','  f ')'").
-Notation "'asubst' '(' v ',' f ',' a ')'" :=
-  (UBinop (UArray2 (USubstElement f)) v a)
-    (in custom koika, v custom koika at level 13, a custom koika at level 13, f constr at level 0, format "'asubst' '(' v ','  f ',' a ')'").
-Notation "'asubstbits' '(' t ',' v ',' f ',' a ')'" :=
-  (UBinop (UArray2 (USubstElementBits t f)) v a)
-    (in custom koika, t constr at level 11, v custom koika at level 13,
-        a custom koika at level 13, f constr at level 0,
-        format "'asubstbits' '(' t ','  v ','  f ',' a ')'").
+Notation "'get' '(' v ',' f ')'"                   := (UUnop  (UStruct1 (UGetField f))           v) (in custom koika, f custom koika_var, format "'get' '(' v ','  f ')'").
+Notation "'getbits' '(' t ',' v ',' f ')'"         := (UUnop  (UStruct1 (UGetFieldBits t f))     v) (in custom koika, f custom koika_var, t constr, format "'getbits' '(' t ','  v ','  f ')'").
+Notation "'subst' '(' v ',' f ',' a ')'"           := (UBinop (UStruct2 (USubstField f))       v a) (in custom koika, f custom koika_var, format "'subst' '(' v ','  f ',' a ')'").
+Notation "'substbits' '(' t ',' v ',' f ',' a ')'" := (UBinop (UStruct2 (USubstFieldBits t f)) v a) (in custom koika, f custom koika_var, t constr, format "'substbits' '(' t ','  v ','  f ',' a ')'").
 
-Declare Custom Entry koika_structs_init.
+Notation "'aref' '(' v ',' f ')'"                   := (UUnop  (UArray1 (UGetElement f))           v) (in custom koika, f constr, format "'aref' '(' v ','  f ')'").
+Notation "'arefbits' '(' t ',' v ',' f ')'"         := (UUnop  (UArray1 (UGetElementBits t f))     v) (in custom koika, f constr, t constr, format "'arefbits' '(' t ','  v ','  f ')'").
+Notation "'asubst' '(' v ',' f ',' a ')'"           := (UBinop (UArray2 (USubstElement f))       v a) (in custom koika, f constr, format "'asubst' '(' v ','  f ',' a ')'").
+Notation "'asubstbits' '(' t ',' v ',' f ',' a ')'" := (UBinop (UArray2 (USubstElementBits t f)) v a) (in custom koika, f constr, t constr, format "'asubstbits' '(' t ','  v ','  f ',' a ')'").
 
-Notation "f ':=' expr" := (cons (f,expr) nil) (in custom koika_structs_init at level 20, f custom koika_var at level 0, expr custom koika at level 88).
-Notation "a ';' b" := (app a b) (in custom koika_structs_init at level 91, a custom koika_structs_init).
-Notation "'struct' structtype '{' fields '}'" :=
-  (USugar (UStructInit structtype fields)) (in custom koika at level 1, structtype constr at level 0, fields custom koika_structs_init at level 92).
-Notation "'struct' structtype '{' '}'" :=
-  (USugar (UStructInit structtype [])) (in custom koika at level 1, structtype constr at level 0).
+(* Koika_branches *)
+Declare Custom Entry koika_branches.
+Notation "x '=>' a "     := [(x,a)]        (in custom koika_branches at level 0, x custom koika at level 200, a custom koika at level 200).
+Notation "arg1 '|' arg2" := (arg1 ++ arg2) (in custom koika_branches at level 1, format "'[v' arg1 ']' '/' '|'  '[v' arg2 ']'").
 
-  Definition mem_req :=
-    {| struct_name := "mem_req";
-       struct_fields := cons ("type", bits_t 1) nil |}.
-
-Notation "'enum' enum_type '{' f '}'" :=
-  (USugar (UConstEnum enum_type f))
-    (in custom koika at level 1, enum_type constr at level 1, f custom koika_var at level 1).
-
+(* TODO total match -> maybe for enums? *)
 Notation "'match' var 'with' '|' branches 'return' 'default' ':' default 'end'" :=
   (USugar (USwitch var default branches))
-    (in custom koika at level 30,
-        var custom koika,
-        branches custom koika_branches,
-        default custom koika at level 99,
+    (in custom koika, branches custom koika_branches,
         format "'match'  var  'with' '/' '[v'  '|'  branches '/' 'return'  'default' ':' default ']' 'end'").
 
-Notation "'#' s" := (USugar (UConstBits s)) (in custom koika at level 98, s constr at level 0, only parsing).
-
+(* ========================================================================= *)
+(*                            scheduler notations                            *)
+(* ========================================================================= *)
 
 Notation "r '|>' s" :=
   (Cons r s)
@@ -266,51 +373,102 @@ Module Type Tests.
   Definition test_20' : uaction reg_t := {{ (yoyo [ magic :+ 3]  ++ yoyo) && yoyo }}.
   Definition test_20'' : uaction reg_t := {{ ( yoyo [ magic :+ 3 ] ++ yoyo ++bla) && yoyo }}.
 
-  (* Notation "'{&' a '&}'" := (a) (a custom koika_types at level 200). *)
-  (* Definition test_21 := {& "yoyo" : bits_t 2 &}. *)
-  (* Definition test_22 := {& "yoyo" : bits_t 2 , "yoyo" : bits_t 2  &}. *)
   Definition test_23 : InternalFunction string string (uaction reg_t) := {{ fun test (arg1 : (bits_t 3)) (arg2 : bits_t 2) : bits_t 4 => magic }}.
   Definition test_24 : nat -> InternalFunction string string (uaction reg_t) :=  (fun sz => {{ fun test (arg1 : bits_t sz) (arg1 : bits_t sz) : bits_t sz  => magic}}).
   Definition test_25 : nat -> InternalFunction string string (uaction reg_t) := (fun sz => {{fun test (arg1 : bits_t sz ) : bits_t sz => let oo := magic >> magic in magic}}).
   Definition test_26 : nat -> InternalFunction string string (uaction reg_t) := (fun sz => {{ fun test () : bits_t sz  => magic }}).
-  Definition test_27 : uaction reg_t :=
-    {{
-        (if (!read0(data0)) then
-           write0(data0, Ob~1);
-             let yo := if (dlk == Ob~1 ) then bla else yoyo || foo
-             in
-             write0(data0, Ob~1)
-         else
-           read0(data0));
-        fail
-    }}.
+  Definition test_27 : uaction reg_t := {{
+    if (!read0(data0)) then
+      write0(data0, Ob~1);
+      let yo := if (dlk == Ob~1 ) then bla else yoyo || foo
+      in
+      write0(data0, Ob~1)
+    else
+      read0(data0);
+    fail
+  }}.
   Definition test_28 : uaction reg_t :=  {{
-                                             match var with
-                                             | magic => magic
-                                             return default: magic
-                                             end
-                                         }}.
+    match var with
+    | magic => magic
+    return default: magic
+    end
+  }}.
 
   Definition mem_req :=
     {| struct_name := "mem_req";
        struct_fields := cons ("type", bits_t 1) nil |}.
 
-  Definition test_30'' : uaction reg_t :=
-    {{
-      struct mem_req { foo := upu[#(Bits.of_nat 3 0) :+ 2] ;
-                       bar := |32`d98| }
-    }}.
+  Definition test_30'' : uaction reg_t := {{
+    struct mem_req { foo := upu[#(Bits.of_nat 3 0) :+ 2] ;
+                     bar := |32`d98| }
+  }}.
 
-  Definition test_31'' : uaction reg_t :=
-    {{
-        pack(a)
-    }}.
+  Definition test_31'' : uaction reg_t := {{
+    pack(a)
+  }}.
 
-  Definition test_31' : uaction reg_t :=
-    {{
-      let a := struct mem_req { foo := upu[#(Bits.of_nat 3 0) :+ 2] ;
-                               bar := |32`d98| } in
-        unpack(struct_t mem_req, pack(a))
-    }}.
+  Definition test_31' : uaction reg_t := {{
+    let a := struct mem_req { foo := upu[#(Bits.of_nat 3 0) :+ 2] ;
+                              bar := |32`d98| } in
+    unpack(struct_t mem_req, pack(a))
+  }}.
+  
+  
+  Notation "'[|' a '=koika=' b '|]'" := ((a : uaction reg_t) = (b : uaction reg_t)) (a custom koika, b custom koika).
+
+  Definition short_get_syntax :
+  [|
+    get(a, some_field)
+  =koika=
+    a.[some_field]
+  |] := eq_refl.
+
+  Definition num_test_b_1 : [| "01101":b     =koika= Ob~0~1~1~0~1 |] := eq_refl.
+  Definition num_test_b_2 : [| 0b"00011"     =koika= Ob~0~0~0~1~1 |] := eq_refl.
+  Definition num_test_b_3 : [| "11":b5       =koika= Ob~0~0~0~1~1 |] := eq_refl.
+  Definition num_test_b_4 : [| 0b"10"5       =koika= Ob~0~0~0~1~0 |] := eq_refl.
+  Definition num_test_b_5 : [| 0b"10010110"3 =koika= Ob~1~1~0     |] := eq_refl.
+  Definition num_test_b_6 : [| "011_01":b    =koika= Ob~0~1~1~0~1 |] := eq_refl.
+  Definition num_test_b_7 : [| "0'11'01":b   =koika= Ob~0~1~1~0~1 |] := eq_refl.
+  Fail Definition num_test_b_6  := {{ 0b"102"  }} : uaction reg_t.
+  Fail Definition num_test_b_7  := {{ 0b"10f"6 }} : uaction reg_t.
+  Fail Definition num_test_b_8  := {{ "f0":b5  }} : uaction reg_t.
+  Fail Definition num_test_b_9  := {{ "f0":b   }} : uaction reg_t.
+  Fail Definition num_test_b_10 := {{ "":b     }} : uaction reg_t.
+
+  Definition num_test_o_1 : [| "330":o   =koika= Ob~0~1~1~0~1~1~0~0~0     |] := eq_refl.
+  Definition num_test_o_2 : [| "070":o9  =koika= Ob~0~0~0~1~1~1~0~0~0     |] := eq_refl.
+  Definition num_test_o_3 : [| 0o"000"   =koika= Ob~0~0~0~0~0~0~0~0~0     |] := eq_refl.
+  Definition num_test_o_4 : [| 0o"750"11 =koika= Ob~0~0~1~1~1~1~0~1~0~0~0 |] := eq_refl.
+  Definition num_test_o_5 : [| 0o"751"3  =koika= Ob~0~0~1                 |] := eq_refl.
+  Fail Definition num_test_o_6  := {{ 0o"108"   }} : uaction reg_t.
+  Fail Definition num_test_o_7  := {{ 0o"080"10 }} : uaction reg_t.
+  Fail Definition num_test_o_8  := {{ "f00":o10 }} : uaction reg_t.
+  Fail Definition num_test_o_9  := {{ "00f":o5  }} : uaction reg_t.
+  Fail Definition num_test_o_10 := {{ "":o      }} : uaction reg_t.
+
+  Definition num_test_d_1 : [| "33":d    =koika= Ob~1~0~0~0~0~1           |] := eq_refl.
+  Definition num_test_d_2 : [| "33":d9   =koika= Ob~0~0~0~1~0~0~0~0~1     |] := eq_refl.
+  Definition num_test_d_3 : [| "070":d9  =koika= Ob~0~0~1~0~0~0~1~1~0     |] := eq_refl.
+  Definition num_test_d_4 : [| 0d"070"   =koika= Ob~1~0~0~0~1~1~0         |] := eq_refl.
+  Definition num_test_d_5 : [| 0d"198"11 =koika= Ob~0~0~0~1~1~0~0~0~1~1~0 |] := eq_refl.
+  Definition num_test_d_6 : [| 0d"15"3   =koika= Ob~1~1~1                 |] := eq_refl.
+  Fail Definition num_test_d_7  := {{ 0d"1a0"   }} : uaction reg_t.
+  Fail Definition num_test_d_8  := {{ 0d"0z0"10 }} : uaction reg_t.
+  Fail Definition num_test_d_9  := {{ "f00":d10 }} : uaction reg_t.
+  Fail Definition num_test_d_10 := {{ "00f":d5  }} : uaction reg_t.
+  Fail Definition num_test_d_11 := {{ "":d      }} : uaction reg_t.
+
+  Definition num_test_h_1 : [| "fa":h    =koika= Ob~1~1~1~1~1~0~1~0         |] := eq_refl.
+  Definition num_test_h_2 : [| "bb":h9   =koika= Ob~0~1~0~1~1~1~0~1~1       |] := eq_refl.
+  Definition num_test_h_3 : [| "014":h   =koika= Ob~0~0~0~0~0~0~0~1~0~1~0~0 |] := eq_refl.
+  Definition num_test_h_4 : [| 0x"070"   =koika= Ob~0~0~0~0~0~1~1~1~0~0~0~0 |] := eq_refl.
+  Definition num_test_h_5 : [| 0x"198"11 =koika= Ob~0~0~1~1~0~0~1~1~0~0~0   |] := eq_refl.
+  Definition num_test_h_6 : [| 0x"1d"3   =koika= Ob~1~0~1                   |] := eq_refl.
+  Definition num_test_h_7 : [| "f_a":h   =koika= Ob~1~1~1~1~1~0~1~0         |] := eq_refl.
+  Fail Definition num_test_h_7  := {{ 0x"1h0"   }} : uaction reg_t.
+  Fail Definition num_test_h_8  := {{ 0x"0z0"10 }} : uaction reg_t.
+  Fail Definition num_test_h_9  := {{ "g00":h10 }} : uaction reg_t.
+  Fail Definition num_test_h_10 := {{ "00k":h5  }} : uaction reg_t.
+  Fail Definition num_test_h_11 := {{ "":h      }} : uaction reg_t.
 End Tests.
-
