coq/IdentParsing.v
@@ -9,6 +9,8 @@ Import Ltac2.Notations.
 Import Coq.Lists.List.ListNotations.
 Open Scope list.
 
+Locate None.
+
 Ltac2 compute c :=
   Std.eval_vm None c.
 
